coq/set/Utils/Decidable.v
@@ -1,3 +1,5 @@
+Require Import Utils.LEM.
+
 (* In this module, we define the notion of decidable predicate: let 'a' be a    *)
 (* type and 'p:a -> Prop' be a predicate. Saying that the predicate 'p' is      *)
 (* decidable is saying 'Dec p' which we are defining as the 'statement':        *)
@@ -28,4 +30,31 @@ Qed.
 
 Arguments Dec2Dec {a} {b} {p}.
 
+(* The notion of decidability is too strong. Let us define a weaker notion.     *)
+Definition Dec'(a:Type) (p:a -> Prop) := forall (x:a), p x \/ ~p x.
 
+Arguments Dec' {a}.
+
+Definition Dec2' (a b:Type) (p:a -> b -> Prop) := 
+    forall (x:a) (y:b), p x y \/ ~p x y.
+
+Arguments Dec2' {a} {b}.
+
+Lemma Dec2Dec' : forall (a b:Type) (p:a -> b -> Prop) (x:a), 
+    Dec2' p -> Dec' (p x).
+Proof.
+    intros a b p x H y. apply H.
+Qed.
+
+(* Weak decidability is weak enough to be implied by LEM.                       *)
+Lemma LEMDec' : LEM -> forall (a:Type) (p:a -> Prop), Dec' p.
+Proof.
+    intros L a p x. apply L.
+Qed.
+
+Arguments LEMDec' _ {a}.
+
+Lemma LEMDec2': LEM -> forall (a b:Type) (p:a -> b -> Prop), Dec2' p.
+Proof.
+    intros L a b p x y. apply L.
+Qed.
