lean/hhg/stmt.lean
@@ -1,6 +1,6 @@
 def State : Type := string → ℕ
 
-def bind (x : string) (n : ℕ) (s:State) : State :=
+def bindVar (x : string) (n : ℕ) (s:State) : State :=
   λ v, if v = x then n else s v
 
 open list
@@ -26,7 +26,7 @@ open stmt
 -- Big step semantics as a relation over State
 inductive BigStep : stmt → State → State → Prop
 | SKIP    : ∀ (s:State), BigStep skip s s
-| ASN     : ∀ (x:string) (a:State → ℕ) (s:State), BigStep (assign x a) s (bind x (a s) s)
+| ASN     : ∀ (x:string) (a:State → ℕ) (s:State), BigStep (assign x a) s (bindVar x (a s) s)
 | SEQ     : ∀ (e₁ e₂:stmt) (s u t:State), BigStep e₁ s u → BigStep e₂ u t → BigStep (e₁ ;; e₂) s t
 | IF_T    : ∀ (p:State → Prop) (e₁ e₂:stmt) (s t:State), p s → BigStep e₁ s t → BigStep (ite p e₁ e₂) s t
 | IF_F    : ∀ (p:State → Prop) (e₁ e₂:stmt) (s t:State), ¬(p s) → BigStep e₂ s t → BigStep (ite p e₁ e₂) s t
@@ -37,13 +37,38 @@ def s0 : State := env [("x",3),("y",5)]
 def s1 : State := env [("x",8),("y",5)]
 def s2 : State := env [("x",8),("y",0)]
 
-def e1 : stmt := assign "x" (λ s, s "x" + s "y") ;; assign "y" (λ s, 0)
+def a0 : State → ℕ := λ s, s "x" + s "y"
+def a1 : State → ℕ := λ _, 0
+
+def e1 : stmt := assign "x" a0 ;; assign "y" a1
+
+lemma L1 : s1 = bindVar "x" (a0 s0) s0 :=
+begin
+  apply funext, unfold s1, unfold s0, unfold a0, unfold env, unfold bindVar,
+  intros s, cases decidable.em (s = "x") with H1 H1,
+    {rewrite H1, simp, cases decidable.em ("y" = "x") with H2 H2,
+      {cases H2},
+      {simp *}},
+    {simp *}
+end
+
+lemma L2 : s2 = bindVar "y" (a1 s1) s1 :=
+begin
+  apply funext, unfold s2, unfold s1, unfold a1, unfold env, unfold bindVar,
+  intros s, cases decidable.em (s = "x") with H1 H1,
+    {rewrite H1, simp, cases decidable.em ("x" = "y") with H2 H2,
+      {cases H2},
+      {simp *}},
+    {simp *, cases decidable.em (s = "y") with H2 H2,
+      {rewrite H2, simp},
+      {simp *}}
+end
 
 open BigStep
 
-lemma L1 : BigStep e1 s0 s2 :=
+lemma L3 : BigStep e1 s0 s2 :=
 begin
   apply (SEQ _ _ s0 s1 s2),
-    {apply (ASN "x" (λ s, s "x" + s "y") s0)},
-    {}
+    {rewrite L1, constructor},
+    {rewrite L2, constructor}
 end
